theory/x64DecodeProof.thy
@@ -5,153 +5,14 @@ imports
   x64Assembler x64Disassembler BitsOpMore BitsOpMore2 BitsOpMore3
   x64DecodeProofAux
 begin
-
+(* It may take more than one hour to run this proof *)
 declare if_split_asm [split]
 
 lemma x64_encode_decode_consistency:
   "list_in_list l_bin pc l \<Longrightarrow> Some l_bin = x64_encode ins \<Longrightarrow>
     x64_decode pc l = Some (length l_bin, ins)"
   apply (cases ins; simp_all)
-                      prefer 6
 
-  subgoal for addr r1 chunk
-    \<comment> \<open> Pmov_mr \<close> 
-      \<comment> \<open> Pmov_rm \<close>
-    apply (cases chunk;simp_all)
-       apply (cases addr ;simp_all)
-    subgoal for base index2 ofs
-      apply (cases base; simp_all)
-      subgoal for base_reg
-        apply (cases index2; simp add: Let_def)
-
-        subgoal \<comment> \<open> ofs < u8 \<and> index2 = None \<and>  not rex \<close>
-          sorry
-          (*apply (cases chunk; simp)
-          apply (unfold construct_rex_to_u8_def construct_modsib_to_u8_def
-              bitfield_insert_u8_def Let_def)
-          using scast_u32_scast_u8_eq
-          apply (cases r1; simp; cases base_reg; simp add: x64_decode_def Let_def ireg_of_u8_def
-                bitfield_insert_u8_def)
-          done*)
-
-        subgoal \<comment> \<open> ofs < u8 \<and> index2 = None \<and> has rex \<close>
-          sorry
-          (*apply (erule conjE;erule conjE)
-          using scast_u32_scast_u8_eq
-          apply (simp add: construct_rex_to_u8_def construct_modsib_to_u8_def
-            bitfield_insert_u8_def Let_def)
-          apply (cases r1; simp_all;erule conjE)
-          apply (cases base_reg;simp_all add: x64_decode_def Let_def ireg_of_u8_def
-                  bitfield_insert_u8_def Suc3_eq_add_3 add.commute)*)
-        done
-      done
-
-
-
-            done
-          subgoal \<comment> \<open> index2 = None  /\ has rex  /\ M64 \<close>
-            apply (cases r1; simp; cases base_reg; simp add: x64_decode_def Let_def ireg_of_u8_def
-                  bitfield_insert_u8_def  Suc3_eq_add_3 add.commute)
-            done
-          done 
-
-        subgoal \<comment> \<open> ofs > u8 /\ index2 = None  /\ not rex \<close>
-          apply (cases chunk; simp; erule conjE)
-          apply (unfold construct_rex_to_u8_def construct_modsib_to_u8_def
-              bitfield_insert_u8_def Let_def)
-
-          using list_in_list_u8_list_of_u32_simp_sym [of ofs "(Suc (Suc pc))" l]
-          using length_u8_list_of_u32_eq_4
-
-          apply (cases dst; simp; cases base_reg; simp add: x64_decode_def Let_def ireg_of_u8_def
-                    bitfield_insert_u8_def Suc3_eq_add_3 add.commute)
-          done 
-
-        subgoal \<comment> \<open> ofs > u8 /\ index2 = None  /\ has rex \<close>
-          apply (cases chunk; simp; erule conjE; erule conjE; erule conjE)
-          apply (unfold construct_rex_to_u8_def construct_modsib_to_u8_def
-              bitfield_insert_u8_def Let_def)
-          subgoal  \<comment> \<open> M32 \<close>
-            using list_in_list_u8_list_of_u32_simp_sym [of ofs "(Suc (Suc (Suc pc)))" l]
-            using length_u8_list_of_u32_eq_4
-            apply (cases dst; simp; cases base_reg; simp add: x64_decode_def Let_def ireg_of_u8_def
-                    bitfield_insert_u8_def Suc3_eq_add_3 Suc4_eq_add_4 add.commute)
-            done
-          subgoal  \<comment> \<open> M64 \<close>
-            using list_in_list_u8_list_of_u32_simp_sym [of ofs "(Suc (Suc (Suc pc)))" l]
-            using length_u8_list_of_u32_eq_4
-            apply (cases dst; simp; cases base_reg; simp add: x64_decode_def Let_def ireg_of_u8_def
-                    bitfield_insert_u8_def Suc3_eq_add_3 Suc4_eq_add_4 add.commute)
-            done
-          done
-
-        subgoal for index22\<comment> \<open> index2 = Some \<close>
-          apply(cases chunk; cases index22;simp_all)
-          subgoal for index_reg scale
-            apply (erule conjE; erule conjE; erule conjE; erule conjE)
-            using list_in_list_u8_list_of_u32_simp_sym [of "ofs" " (Suc (Suc (Suc (Suc pc))))" l]
-            using length_u8_list_of_u32_eq_4
-            using construct_modsib_to_u8_imply_index_reg [of " (and (u8_of_ireg dst) 8 \<noteq> 0)" index_reg base_reg "l ! pc" scale "l ! (Suc (Suc (Suc pc)))"]
-            using construct_modsib_to_u8_imply_base_reg  [of " (and (u8_of_ireg dst) 8 \<noteq> 0)" index_reg base_reg "l ! pc" scale "l ! (Suc (Suc (Suc pc)))"]
-            using construct_modsib_to_u8_imply_scale [of scale index_reg base_reg "l !  Suc (Suc (Suc pc))"]
-              apply (cases dst; simp add: construct_rex_to_u8_def  construct_modsib_to_u8_def)
-              subgoal by (cases base_reg; simp; cases index_reg; simp add: x64_decode_def
-                     bitfield_insert_u8_def Let_def ireg_of_u8_def
-                    add.commute Suc3_eq_add_3 Suc4_eq_add_4) 
-              subgoal by (cases base_reg; simp; cases index_reg; simp add: x64_decode_def
-                     bitfield_insert_u8_def Let_def ireg_of_u8_def
-                    add.commute Suc3_eq_add_3 Suc4_eq_add_4) 
-              subgoal by (cases base_reg; simp; cases index_reg; simp add: x64_decode_def
-                     bitfield_insert_u8_def Let_def ireg_of_u8_def
-                    add.commute Suc3_eq_add_3 Suc4_eq_add_4) 
-              subgoal by (cases base_reg; simp; cases index_reg; simp add: x64_decode_def
-                     bitfield_insert_u8_def Let_def ireg_of_u8_def
-                    add.commute Suc3_eq_add_3 Suc4_eq_add_4) 
-              subgoal by (cases base_reg; simp; cases index_reg; simp add: x64_decode_def
-                     bitfield_insert_u8_def Let_def ireg_of_u8_def
-                    add.commute Suc3_eq_add_3 Suc4_eq_add_4) 
-              subgoal by (cases base_reg; simp; cases index_reg; simp add: x64_decode_def
-                     bitfield_insert_u8_def Let_def ireg_of_u8_def
-                    add.commute Suc3_eq_add_3 Suc4_eq_add_4) 
-              subgoal by (cases base_reg; simp; cases index_reg; simp add: x64_decode_def
-                     bitfield_insert_u8_def Let_def ireg_of_u8_def
-                    add.commute Suc3_eq_add_3 Suc4_eq_add_4) 
-              subgoal by (cases base_reg; simp; cases index_reg; simp add: x64_decode_def
-                     bitfield_insert_u8_def Let_def ireg_of_u8_def
-                    add.commute Suc3_eq_add_3 Suc4_eq_add_4) 
-              subgoal by (cases base_reg; simp; cases index_reg; simp add: x64_decode_def
-                     bitfield_insert_u8_def Let_def ireg_of_u8_def
-                    add.commute Suc3_eq_add_3 Suc4_eq_add_4) 
-              subgoal by (cases base_reg; simp; cases index_reg; simp add: x64_decode_def
-                     bitfield_insert_u8_def Let_def ireg_of_u8_def
-                    add.commute Suc3_eq_add_3 Suc4_eq_add_4) 
-              subgoal by (cases base_reg; simp; cases index_reg; simp add: x64_decode_def
-                     bitfield_insert_u8_def Let_def ireg_of_u8_def
-                    add.commute Suc3_eq_add_3 Suc4_eq_add_4) 
-              subgoal by (cases base_reg; simp; cases index_reg; simp add: x64_decode_def
-                     bitfield_insert_u8_def Let_def ireg_of_u8_def
-                    add.commute Suc3_eq_add_3 Suc4_eq_add_4) 
-              subgoal by (cases base_reg; simp; cases index_reg; simp add: x64_decode_def
-                     bitfield_insert_u8_def Let_def ireg_of_u8_def
-                    add.commute Suc3_eq_add_3 Suc4_eq_add_4) 
-              subgoal by (cases base_reg; simp; cases index_reg; simp add: x64_decode_def
-                     bitfield_insert_u8_def Let_def ireg_of_u8_def
-                    add.commute Suc3_eq_add_3 Suc4_eq_add_4) 
-              subgoal by (cases base_reg; simp; cases index_reg; simp add: x64_decode_def
-                     bitfield_insert_u8_def Let_def ireg_of_u8_def
-                    add.commute Suc3_eq_add_3 Suc4_eq_add_4) 
-              subgoal by (cases base_reg; simp; cases index_reg; simp add: x64_decode_def
-                     bitfield_insert_u8_def Let_def ireg_of_u8_def
-                    add.commute Suc3_eq_add_3 Suc4_eq_add_4) 
-            done
-          done
-        done
-      done
-    done
-
-
-
-(*
   subgoal for dst src
   \<comment> \<open> Pmovl_rr \<close> 
     apply (unfold Let_def)
@@ -320,10 +181,142 @@ lemma x64_encode_decode_consistency:
     done
 
 
-  subgoal for dst src chunk
+  subgoal for addr r1 chunk
     \<comment> \<open> Pmov_mr \<close> 
-    sorry
+      \<comment> \<open> Pmov_rm \<close>
+    apply (cases addr ;simp_all)
+    subgoal for base index2 ofs
+      apply (cases base; simp_all)
+      subgoal for base_reg
+        apply (cases index2; simp add: Let_def)
 
+        subgoal \<comment> \<open> ofs < u8 \<and> index2 = None \<and>  not rex \<close>
+        using scast_u32_scast_u8_eq
+          apply (cases chunk; simp_all add:construct_rex_to_u8_def construct_modsib_to_u8_def
+              bitfield_insert_u8_def Let_def)
+          apply (erule conjE; erule conjE)
+          subgoal by(cases r1; simp; cases base_reg; simp add: x64_decode_def Let_def ireg_of_u8_def
+                bitfield_insert_u8_def )
+          subgoal by(cases r1; simp; cases base_reg; simp add: x64_decode_def Let_def ireg_of_u8_def
+                bitfield_insert_u8_def  Suc3_eq_add_3 add.commute)
+          subgoal by(cases r1; simp; cases base_reg; simp add: x64_decode_def Let_def ireg_of_u8_def
+                bitfield_insert_u8_def )
+          done
+
+
+        subgoal \<comment> \<open> ofs < u8 \<and> index2 = None \<and> has rex \<close>
+          using scast_u32_scast_u8_eq
+          apply (cases chunk; simp_all add:construct_rex_to_u8_def construct_modsib_to_u8_def
+              bitfield_insert_u8_def Let_def)
+               apply (erule conjE; erule conjE;erule conjE)
+          subgoal
+            by (cases r1; simp; cases base_reg;simp_all add: x64_decode_def Let_def ireg_of_u8_def
+                  bitfield_insert_u8_def Suc3_eq_add_3 add.commute )
+          subgoal
+            by (cases r1; simp; cases base_reg; simp add: x64_decode_def Let_def ireg_of_u8_def
+                bitfield_insert_u8_def  Suc3_eq_add_3 add.commute)
+          subgoal
+            by (cases r1; simp; cases base_reg; simp add: x64_decode_def Let_def ireg_of_u8_def
+                bitfield_insert_u8_def  Suc3_eq_add_3 add.commute)
+          subgoal
+            by (cases r1; simp; cases base_reg; simp add: x64_decode_def Let_def ireg_of_u8_def
+                bitfield_insert_u8_def  Suc3_eq_add_3 add.commute)
+            done
+
+
+
+        subgoal \<comment> \<open> ofs > u8 /\ index2 = None  /\ not rex \<close>
+          apply (cases chunk; simp; erule conjE)
+          apply (unfold construct_rex_to_u8_def construct_modsib_to_u8_def; erule conjE)
+
+          using list_in_list_u8_list_of_u32_simp_sym [of ofs "(Suc (Suc pc))" l]
+          using length_u8_list_of_u32_eq_4
+
+          apply (cases r1; simp; cases base_reg; simp add: x64_decode_def Let_def ireg_of_u8_def
+                    bitfield_insert_u8_def Suc3_eq_add_3 add.commute)
+          done 
+
+        subgoal \<comment> \<open> ofs > u8 /\ index2 = None  /\ has rex \<close>
+          apply (cases chunk; simp; erule conjE; erule conjE; erule conjE)
+          apply (unfold construct_rex_to_u8_def construct_modsib_to_u8_def
+              bitfield_insert_u8_def Let_def)
+          subgoal  \<comment> \<open> M32 \<close>
+            using list_in_list_u8_list_of_u32_simp_sym [of ofs "(Suc (Suc (Suc pc)))" l]
+            using length_u8_list_of_u32_eq_4
+            apply (cases r1; simp; cases base_reg; simp add: x64_decode_def Let_def ireg_of_u8_def
+                    bitfield_insert_u8_def Suc3_eq_add_3 Suc4_eq_add_4 add.commute)
+            done
+          subgoal  \<comment> \<open> M64 \<close>
+            using list_in_list_u8_list_of_u32_simp_sym [of ofs "(Suc (Suc (Suc pc)))" l]
+            using length_u8_list_of_u32_eq_4
+            apply (cases r1; simp; cases base_reg; simp add: x64_decode_def Let_def ireg_of_u8_def
+                    bitfield_insert_u8_def Suc3_eq_add_3 Suc4_eq_add_4 add.commute)
+            done
+          done
+
+        subgoal for index22\<comment> \<open> index2 = Some \<close>
+          apply(cases chunk; cases index22;simp_all)
+          subgoal for index_reg scale
+            apply (erule conjE; erule conjE; erule conjE; erule conjE)
+            using list_in_list_u8_list_of_u32_simp_sym [of "ofs" " (Suc (Suc (Suc (Suc pc))))" l]
+            using length_u8_list_of_u32_eq_4
+            using construct_modsib_to_u8_imply_index_reg [of " (and (u8_of_ireg r1) 8 \<noteq> 0)" index_reg base_reg "l ! pc" scale "l ! (Suc (Suc (Suc pc)))"]
+            using construct_modsib_to_u8_imply_base_reg  [of " (and (u8_of_ireg r1) 8 \<noteq> 0)" index_reg base_reg "l ! pc" scale "l ! (Suc (Suc (Suc pc)))"]
+            using construct_modsib_to_u8_imply_scale [of scale index_reg base_reg "l !  Suc (Suc (Suc pc))"]
+              apply (cases r1; simp add: construct_rex_to_u8_def  construct_modsib_to_u8_def)
+              subgoal by (cases base_reg; simp; cases index_reg; simp add: x64_decode_def
+                     bitfield_insert_u8_def Let_def ireg_of_u8_def
+                    add.commute Suc3_eq_add_3 Suc4_eq_add_4) 
+              subgoal by (cases base_reg; simp; cases index_reg; simp add: x64_decode_def
+                     bitfield_insert_u8_def Let_def ireg_of_u8_def
+                    add.commute Suc3_eq_add_3 Suc4_eq_add_4) 
+              subgoal by (cases base_reg; simp; cases index_reg; simp add: x64_decode_def
+                     bitfield_insert_u8_def Let_def ireg_of_u8_def
+                    add.commute Suc3_eq_add_3 Suc4_eq_add_4) 
+              subgoal by (cases base_reg; simp; cases index_reg; simp add: x64_decode_def
+                     bitfield_insert_u8_def Let_def ireg_of_u8_def
+                    add.commute Suc3_eq_add_3 Suc4_eq_add_4) 
+              subgoal by (cases base_reg; simp; cases index_reg; simp add: x64_decode_def
+                     bitfield_insert_u8_def Let_def ireg_of_u8_def
+                    add.commute Suc3_eq_add_3 Suc4_eq_add_4) 
+              subgoal by (cases base_reg; simp; cases index_reg; simp add: x64_decode_def
+                     bitfield_insert_u8_def Let_def ireg_of_u8_def
+                    add.commute Suc3_eq_add_3 Suc4_eq_add_4) 
+              subgoal by (cases base_reg; simp; cases index_reg; simp add: x64_decode_def
+                     bitfield_insert_u8_def Let_def ireg_of_u8_def
+                    add.commute Suc3_eq_add_3 Suc4_eq_add_4) 
+              subgoal by (cases base_reg; simp; cases index_reg; simp add: x64_decode_def
+                     bitfield_insert_u8_def Let_def ireg_of_u8_def
+                    add.commute Suc3_eq_add_3 Suc4_eq_add_4) 
+              subgoal by (cases base_reg; simp; cases index_reg; simp add: x64_decode_def
+                     bitfield_insert_u8_def Let_def ireg_of_u8_def
+                    add.commute Suc3_eq_add_3 Suc4_eq_add_4) 
+              subgoal by (cases base_reg; simp; cases index_reg; simp add: x64_decode_def
+                     bitfield_insert_u8_def Let_def ireg_of_u8_def
+                    add.commute Suc3_eq_add_3 Suc4_eq_add_4) 
+              subgoal by (cases base_reg; simp; cases index_reg; simp add: x64_decode_def
+                     bitfield_insert_u8_def Let_def ireg_of_u8_def
+                    add.commute Suc3_eq_add_3 Suc4_eq_add_4) 
+              subgoal by (cases base_reg; simp; cases index_reg; simp add: x64_decode_def
+                     bitfield_insert_u8_def Let_def ireg_of_u8_def
+                    add.commute Suc3_eq_add_3 Suc4_eq_add_4) 
+              subgoal by (cases base_reg; simp; cases index_reg; simp add: x64_decode_def
+                     bitfield_insert_u8_def Let_def ireg_of_u8_def
+                    add.commute Suc3_eq_add_3 Suc4_eq_add_4) 
+              subgoal by (cases base_reg; simp; cases index_reg; simp add: x64_decode_def
+                     bitfield_insert_u8_def Let_def ireg_of_u8_def
+                    add.commute Suc3_eq_add_3 Suc4_eq_add_4) 
+              subgoal by (cases base_reg; simp; cases index_reg; simp add: x64_decode_def
+                     bitfield_insert_u8_def Let_def ireg_of_u8_def
+                    add.commute Suc3_eq_add_3 Suc4_eq_add_4) 
+              subgoal by (cases base_reg; simp; cases index_reg; simp add: x64_decode_def
+                     bitfield_insert_u8_def Let_def ireg_of_u8_def
+                    add.commute Suc3_eq_add_3 Suc4_eq_add_4) 
+            done
+          done
+        done
+      done
+    done
 
   subgoal for addr imm chunk
     \<comment> \<open> Pmov_mi \<close> 
@@ -1102,6 +1095,6 @@ lemma x64_encode_decode_consistency:
   subgoal 
     \<comment> \<open> Pnop \<close>
     apply(unfold Let_def x64_decode_def; simp)
-    done*)
+    done
   done
 end
